src/Language/PlutusIR/Transform/ThunkRecursions.v
@@ -1,20 +1,215 @@
+From Coq Require Import
+  Strings.String
+  Lists.List
+.
+
 From PlutusCert Require Import
   Language.PlutusIR
+  Analysis.BoundVars
+  Transform.Congruence
+  Semantics.Dynamic.Values
+  Util.List
   .
+
 Import NamedTerm.
-
-
-Polymorphic Inductive ThunkRecursions : Term -> Term -> Type := .
-
+Import ListNotations.
 
 (*
-All recursive definitions that are not of function type are thunked: this is a hack to make it compatible with fixpoint combinator
-  , which requires a function type. Examples:
-    - a polymorphic function like map
-    - a recursive Int: x :: Int = x + x
-        (Hmm, a strict binding here should not terminate, does the compiler consider this case?
-         It seems like I can't generate a strict binding of non-function type that diverges:
-         plutus generates nonstrict lets for expressions that are not values (it seems?))
-         If only values result in strict let bindings, what is the point of having strict bindings?
-    - a polymorphic value like x :: forall a. [[a]] = [] : x)
+
+Summary
+---
+
+Strict Let Rec bindings that don't have a function type will be thunked so that
+their type is of function type (unit -> τ). For example polymorphic functions
+(∀a ∀b. ...). This is necessary for the compilation step that translates Let Rec
+using the indexed fixpoint combinator, which can only handle recursive bindings
+with function type.
+
+This pass doesn't actually do thunking, it just changes strict bindings to
+non-strict so that the later LetNonStrict pass will thunk them. An additional
+(shadowing) strict binder is then added to "strictify" the term again.
+
+In other words, this pass should establish the post-condititon that all LetRec
+bindings have function type.
+
+Global uniqueness
+---
+According to [1], this pass does not preserve global uniquness, because
+each thunked recursive binder will have a non-recursive "adapter" binder with
+the same name.
+
+[1] plutus-core/plutus-ir/src/PlutusIR/Transform/ThunkRecursions.hs
+
+
+Possibly implement as function
+---
+
+The relation below is more general, because it allows the transformation to be
+optionally applied. However, in the compiler, this is not optional, and all
+strict letrecs with non-function type are transformed.
+
+We could implement this in coq as a function which should result in a syntactic
+equivalent term (there will be no new binder names).
+
 *)
+
+
+
+(* Records each binder in the Let Rec that was unstrictified *)
+
+Inductive binder_info := let_bound : Strictness -> binder_info | lambda_bound.
+
+Definition ctx := list (string * binder_info).
+
+Definition ctx_unstrictified := list (string * (Term * ctx)).
+
+Definition Binding_to_ctx (b : Binding) : ctx :=
+  match b with
+    | TermBind s (VarDecl x τ) t => [(x, let_bound s)]
+    | _ => []
+  end
+.
+
+
+(* Similar to mkLet in Plutus: for an empty list of bindings it is the identity, otherwise
+   it constructs a let with a non-empty list of bindings *)
+Definition mk_let (r : Recursivity) (bs : list Binding) (t : Term) : Term :=
+  match bs with
+    | [] => t
+    | _  => Let r bs t
+  end
+.
+
+(* Pure values do not need to be strictified after non-strictification *)
+Inductive is_pure (Γ : ctx) : Term -> Type :=
+
+  | is_pure_value : forall t,
+      value t ->
+      ~(is_error t) ->
+      is_pure Γ t
+
+  | is_pure_var_let : forall x,
+      Lookup x (let_bound Strict) Γ ->
+      is_pure Γ (Var x)
+
+  | is_pure_var_lambda : forall x,
+      Lookup x lambda_bound Γ ->
+      is_pure Γ (Var x)
+.
+
+
+
+Inductive thunk_rec (Γ : ctx) : Term -> Term -> Type :=
+
+  | tr_Let_Rec : forall bs bs' t t' Γ_bs bs_new Ω,
+      thunk_rec_Bindings_Rec (Γ_bs ++ Γ) bs bs' Ω ->
+      thunk_rec (Γ_bs ++ Γ) t t' ->
+      strictify Γ Ω bs_new ->
+      thunk_rec Γ (Let Rec bs t) (Let Rec bs' (mk_let NonRec bs_new t'))
+
+  (* Congruence cases, `Cong` cannot currently capture
+     this pattern, which has to extend the ctx Γ in all 
+     term binders *)
+  | tr_Let_NonRec : forall bs bs' t t' Γ_bs,
+     thunk_rec_Bindings_NonRec Γ bs bs' Γ_bs ->
+     thunk_rec (Γ_bs ++ Γ) t t' ->
+     thunk_rec Γ (Let Rec bs t) (Let Rec bs' t')
+  | tr_Var      : forall x,
+      thunk_rec Γ (Var x) (Var x)
+  | tr_TyAbs    : forall α k t t',
+      thunk_rec Γ t t' ->
+      thunk_rec Γ (TyAbs α k t) (TyAbs α k t')
+  | tr_LamAbs   : forall x τ t t',
+      thunk_rec ((x, lambda_bound) :: Γ) t t' ->
+      thunk_rec Γ (LamAbs x τ t) (LamAbs x τ t')
+  | tr_Apply    : forall s s' t t',
+      thunk_rec Γ s s' ->
+      thunk_rec Γ t t' ->
+      thunk_rec Γ (Apply s t) (Apply s' t')
+  | tr_Constant : forall c,
+      thunk_rec Γ (Constant c) (Constant c)
+  | tr_Builtin  : forall f,
+      thunk_rec Γ (Builtin f) (Builtin f)
+  | tr_TyInst   : forall t t' τ,
+      thunk_rec Γ t t' ->
+      thunk_rec Γ (TyInst t τ) (TyInst t' τ)
+  | tr_Error    : forall τ,
+      thunk_rec Γ (Error τ) (Error τ)
+  | tr_IWrap    : forall σ τ t t',
+      thunk_rec Γ (IWrap σ τ t) (IWrap σ τ t')
+  | tr_Unwrap   : forall t t',
+      thunk_rec Γ (Unwrap t) (Unwrap t')
+
+with thunk_rec_Bindings_NonRec (Γ : ctx) : list Binding -> list Binding -> ctx -> Type :=
+
+  | tr_Bindings_NonRec_nil :
+      thunk_rec_Bindings_NonRec Γ [] [] Γ
+
+  | tr_Bindings_NonRec_cons : forall b b' bs bs',
+      forall Γ_b Γ_bs,
+        thunk_rec_Binding_NonRec  Γ b b' ->
+        thunk_rec_Bindings_NonRec (Binding_to_ctx b ++ Γ) bs bs' Γ_bs ->
+        thunk_rec_Bindings_NonRec Γ (b :: bs) (b' :: bs') (Γ_bs ++ Γ_b)
+
+
+with thunk_rec_Bindings_Rec (Γ : ctx) : list Binding -> list Binding -> ctx_unstrictified -> Type :=
+
+  | tr_Bindings_Rec_nil :
+      thunk_rec_Bindings_Rec Γ [] [] []
+
+  | tr_Bindings_Rec_cons : forall b b' bs bs' Ω_b Ω_bs,
+      thunk_rec_Binding_Rec Γ b b' Ω_b ->
+      thunk_rec_Bindings_Rec Γ bs bs' Ω_bs->
+      thunk_rec_Bindings_Rec Γ (b :: bs) (b' :: bs') (Ω_bs ++ Ω_b)
+
+(* Also indexed by the unstrictified bindings *)
+with thunk_rec_Binding_NonRec (Γ : ctx) : Binding -> Binding -> Type :=
+
+  | tr_TermBind_NonRec : forall s vd t t',
+      thunk_rec Γ t t' ->
+      thunk_rec_Binding_NonRec Γ (TermBind s vd t) (TermBind NonStrict vd t')
+
+  | tr_DatatypeBind_NonRec : forall d,
+      thunk_rec_Binding_NonRec Γ (DatatypeBind d) (DatatypeBind d)
+
+  | tr_TypeBind_NonRec : forall tvd τ,
+      thunk_rec_Binding_NonRec Γ (TypeBind tvd τ) (TypeBind tvd τ)
+
+(* Also indexed by the unstrictified bindings *)
+with thunk_rec_Binding_Rec (Γ : ctx) : Binding -> Binding -> ctx_unstrictified -> Type :=
+
+  (* The actual implementation only unstrictifies non-function type bindings, but
+     it is a sound transformation for any strict recursive binding *)
+  | tr_TermBind_Rec_Unstrictify : forall vd t t' x τ,
+      thunk_rec Γ t t' ->
+      vd = VarDecl x τ ->
+      thunk_rec_Binding_Rec Γ (TermBind Strict vd t) (TermBind NonStrict vd t') [(x, (t, Γ))]
+
+  | tr_TermBind_Rec : forall s vd t t',
+      thunk_rec Γ t t' ->
+      thunk_rec_Binding_Rec Γ (TermBind s vd t) (TermBind s vd t') []
+
+  | tr_DatatypeBind_Rec : forall d,
+      thunk_rec_Binding_Rec Γ (DatatypeBind d) (DatatypeBind d) []
+
+  | tr_TypeBind_Rec : forall tvd τ,
+      thunk_rec_Binding_Rec Γ (TypeBind tvd τ) (TypeBind tvd τ) []
+
+(* Add let NonRec bindings for unstrictified bindings, except if
+   they were definitely pure *)
+with strictify (Γ : ctx) : ctx_unstrictified -> list Binding -> Type :=
+
+  | str_cons_pure : forall Γ_t t x Ω_bs bs,
+     is_pure Γ_t t ->
+     strictify Γ                 Ω_bs  bs ->
+     strictify Γ ((x, (t, Γ)) :: Ω_bs) bs
+
+  | str_cons_strictify : forall x x_info τ b bs Ω_bs,
+     Lookup x (let_bound Strict) Γ ->
+     b = TermBind Strict (VarDecl x τ) (Var x) ->
+     strictify Γ                 Ω_bs         bs ->
+     strictify Γ ((x, x_info) :: Ω_bs) ((b :: bs))
+
+  | str_nil :
+     strictify Γ [] []
+.
